thys/Collections/Refine_Dflt_Only_ICF.thy
@@ -10,19 +10,20 @@ text {* Contains the Monadic Refinement Framework and the original
   Isabelle Collection Framework. The generic collection framework is
   not included *}
 
-declaration {* let open Autoref_Fix_Rel in fn phi =>
-  I 
-  #> declare_prio "RBT-set" @{cpat "\<langle>?R\<rangle>rs.rel"} PR_LAST phi
-  #> declare_prio "Hash-set" @{cpat "\<langle>?R\<rangle>hs.rel"} PR_LAST phi
-  #> declare_prio "List-set" @{cpat "\<langle>?R\<rangle>lsi.rel"} PR_LAST phi
-end *}
+local_setup {*
+  let open Autoref_Fix_Rel in
+    declare_prio "RBT-set" @{term "\<langle>R\<rangle>rs.rel"} PR_LAST #>
+    declare_prio "Hash-set" @{term "\<langle>R\<rangle>hs.rel"} PR_LAST #>
+    declare_prio "List-set" @{term "\<langle>R\<rangle>lsi.rel"} PR_LAST
+  end
+*}
 
-declaration {* let open Autoref_Fix_Rel in fn phi =>
-  I 
-  #> declare_prio "RBT-map" @{cpat "\<langle>?Rk,?Rv\<rangle>rm.rel"} PR_LAST phi
-  #> declare_prio "Hash-map" @{cpat "\<langle>?Rk,?Rv\<rangle>hm.rel"} PR_LAST phi
-  #> declare_prio "List-map" @{cpat "\<langle>?Rk,?Rv\<rangle>lmi.rel"} PR_LAST phi
-end *}
-
+local_setup {*
+  let open Autoref_Fix_Rel in
+    declare_prio "RBT-map" @{term "\<langle>Rk,Rv\<rangle>rm.rel"} PR_LAST #>
+    declare_prio "Hash-map" @{term "\<langle>Rk,Rv\<rangle>hm.rel"} PR_LAST #>
+    declare_prio "List-map" @{term "\<langle>Rk,Rv\<rangle>lmi.rel"} PR_LAST
+  end
+*}
 
 end
